\documentclass[11pt]{article}
\usepackage[a4paper, margin=1in]{geometry}
\usepackage{amsmath, amssymb, amsthm}
\usepackage{tikz-cd}
\usepackage{mathrsfs}

\newcommand{\comp}{\circ}
\newcommand{\id}{\mathrm{id}}

\renewcommand{\qedsymbol}{$\blacksquare$}
\begin{document}

\begin{table}[ht]
\centering
\renewcommand{\arraystretch}{2.2}
\setlength{\tabcolsep}{6pt}
\section{Universal Constructions}
\resizebox{\textwidth}{!}{%
\begin{tabular}{|l|c|l|c|c|}
  \hline
  
Construction & Definition & Computation & Equality & Commutative Diagram \\ \hline
Initial Object &
$\frac{}{0 \xrightarrow{[]} A}$ &
 &
$\frac{f: 0 \to A}{f = []}$ &
\begin{tikzcd}[ampersand replacement=\&, baseline=(current bounding box.center)] 0 \arrow[r, "{[]}", dotted] \& A \end{tikzcd} \\ \hline
Terminal Object &
$\frac{A}{A \xrightarrow{\langle \rangle} 1}$ &
 &
$\frac{f: A \to 1}{f = \langle \rangle}$ &
\begin{tikzcd}[ampersand replacement=\&, baseline=(current bounding box.center)] A \arrow[r, "{\langle \rangle}", dotted] \& 1 \end{tikzcd} \\ \hline
Products &
$\frac{A \xrightarrow{f} X \quad A \xrightarrow{g} Y}{A \xrightarrow{\langle f,g \rangle} X \times Y}$ &
\begin{tabular}{@{}l@{}}
$\pi_1 \comp \langle f,g \rangle = f, \pi_2 \comp \langle f,g \rangle = g$ \\
$\langle \pi_1, \pi_2 \rangle \comp h = h : A \to X \times Y$
\end{tabular} &
$\frac{\pi_1 \comp h = f : A \to X \quad \pi_2 \comp h = g : A \to Y}{h = \langle f,g \rangle : A \to X \times Y}$ &
\begin{tikzcd}[ampersand replacement=\&, baseline=(current bounding box.center), row sep=small, column sep=small]
\& A \arrow[ld, "f"'] \arrow[rd, "g"] \arrow[d, "{\langle f,g \rangle}", dotted] \& \\
X \& X \times Y \arrow[l, "\pi_1"] \arrow[r, "\pi_2"'] \& Y
\end{tikzcd} \\ \hline
Coproducts &
$\frac{A \xrightarrow{f} X \quad B \xrightarrow{g} X}{A + B \xrightarrow{[f,g]} X}$ &
\begin{tabular}{@{}l@{}}
$[f,g] \comp \iota_1 = f, [f,g] \comp \iota_2 = g$ \\
$[h \comp \iota_1, h \comp \iota_2] = h : A + B \to X$
\end{tabular} &
$\frac{h \comp \iota_1 = f : A \to X \quad h \comp \iota_2 = g : B \to X}{h = [f,g] : A + B \to X}$ &
\begin{tikzcd}[ampersand replacement=\&, baseline=(current bounding box.center), row sep=small, column sep=small]
A \arrow[r, "\iota_1"] \arrow[rd, "f"'] \& A + B \arrow[d, "{[f,g]}", dotted] \& B \arrow[l, "\iota_2"'] \arrow[ld, "g"] \\
\& X \&
\end{tikzcd} \\ \hline
Exponentials &
$\frac{A \times X \xrightarrow{f} Y}{A \xrightarrow{\text{cur}f} X \Rightarrow Y}$ &
\begin{tabular}{@{}l@{}}
$\text{app} \comp (\text{cur}f \times \id_X) = f : A \times X \to Y$ \\
$\text{cur}(\text{app} \comp (h \times \id_X)) = h : A \to X \Rightarrow Y$
\end{tabular} &
$\frac{\text{app} \comp (h \times \id_X) = f : A \times X \to Y}{h = \text{cur}f : A \to X \Rightarrow Y}$ &
\begin{tikzcd}[ampersand replacement=\&, baseline=(current bounding box.center), row sep=small, column sep=small]
A \times X \arrow[rr, "{\text{cur}f \times \id}", dotted] \arrow[rd, "f"'] \& \& (X \Rightarrow Y) \times X \arrow[ld, "\text{app}"] \\
\& Y \&
\end{tikzcd} \\ \hline
Free monoids &
$\frac{X \xrightarrow{f} M \in \underline{\text{Set}}}{\underline{L}X \xrightarrow{f^\sharp}\underline{M} \in \underline{\text{Mon}}}$ &
\begin{tabular}{@{}l@{}}
$f^\sharp \comp s_X = f : X \to M$ \\
$(g \comp s_X)^\sharp = g : \underline{L}X \to \underline{M}$
\end{tabular} &
$\frac{h \comp s_X = f : X \to M}{h = f^\sharp : \underline{L}X \to \underline{M}}$ &
\begin{tikzcd}[ampersand replacement=\&, baseline=(current bounding box.center), row sep=small, column sep=small]
X \arrow[r, "s_X"] \arrow[rd, "f"'] \& \underline{L}X \arrow[d, "f^\sharp", dotted] \\
\& \underline{M}
\end{tikzcd} \\ \hline
\end{tabular}%
}
\end{table}

\section{Equational Reasoning Laws}

\[f = \langle \rangle : X \to 1_C\]
\[k = \langle f, g \rangle \iff (\pi_1 \circ k = f \land \pi_2 \circ k = g) : X \to Y \times Z\]
\[\pi_1 \circ (f \times g) = f \circ \pi_1 : X \times Y \to X_2\]
\[\pi_2 \circ (f \times g) = g \circ \pi_2 : X \times Y \to Y_2\]
\[\langle \pi_1, \pi_2, \rangle = id_{X \times Y} : X \times Y \to X \times Y\]
\[id_X \times id_Y = id_{X \times Y} : X \times Y \to X \times Y\]
\[(h \times k) \circ (f \times g) = (h \circ f) \times (k \circ g) : X_1 \times Y_1 \to X_3 \times Y_3\]
\[f = g \iff cur(f) = cur(g)\]
\[(g = cur(f)) \iff f = app \circ (g \times id)\]
\[cur(app) = id_{X \implies Y} : X \implies Y \to X \implies Y \]
\[\langle g_1, g_2 \rangle \circ f = \langle g_1 \circ f , g_2 \circ f \rangle\]
\[(f_1 \times f_2) \circ \langle g_1 , g_2 \rangle = \langle f_1 \circ g_1, f_2 \circ g_2 \rangle\]



\[u : X \to Y, g : F(Y) \to Z, v : Z \to W\]
\[\theta_{X, W}(v \circ g \circ F(u)) = G(v) \circ \theta_{Y,Z}(g) \circ u\]
\[\theta_{X, W}(g \circ F(u)) = \theta_{Y,Z}(g) \circ u\]
\[\theta_{X, W}(v \circ g) = G(v) \circ \theta_{Y,Z}(g)\]

\[u : X \to Y, g : Y \to G(Z), v : Z \to W\]
\[\theta^{-1}_{X, W}(G(v) \circ g \circ u) = v \circ \theta^{-1}_{Y,Z}(g) \circ F(u)\]
\[\theta^{-1}_{X, W}(g \circ u) = \theta^{-1}_{Y,Z}(g) \circ F(u)\]
\[\theta^{-1}_{X, W}(G(v) \circ g) = v \circ \theta^{-1}_{Y,Z}(g)\]


\section{Categories}
\section{Functors}
\section{Natural Transformations}
\[\eta : Id_C \to GF\]
\[ \eta_X = \theta_{X, FX}(id_{FX}) \]

\[\varepsilon : FG \to Id_D\]
\[\varepsilon_X = \theta^{-1}_{GX, X}(id_{GX}) \]

\[\theta(f : A \to G(B)) = \varepsilon_B \circ F(f) : F(A) \to B\]
\[\theta^{-1}(g : F(A) \to B) = G(g) \circ \eta_A : A \to G(B)\]
\subsection{Triangle Identity}
\[\varepsilon_F \circ F\eta = id_F\]
\[G\varepsilon \circ \eta_G = id_G\]

\section{Adjunctions}
\section{cartesian closed structure}
\section{left and right adjoints}
\section{dependent products and functions}
\section{exponentials in presheaf categories}

\subsection{Presheave category}
Objects: contravariant functors \[P : C^{op} \to Set\]
Arrows: natural transformations

\subsubsection{Exponential Object}
$$(G^F)(U) \cong \text{Nat}(F \times \text{Hom}(-, U), G)$$
Action on objects: $$(Y^X)(C) = \text{Nat}(\mathbf{y}(C) \times X, Y)$$
Action on arrows:
$$ (Y^X)(f): (Y^X)(C) \to (Y^X)(C') $$
\[ (Y^X)(f)(\phi)_W(g, x) = \phi_w(f \circ g, x)$\]
Yoneda Functor:
\[Y : C \to Set^{C^{op}}\]
\[Y(A : C) = \mathbb{C}(\cdot, A)\]

Yoneda Lemma:
\[Set^{C^{op}}(Y(X), P) \equiv P(X)\]
Where
\[P : C^{op} \to Set\]

\end{document}
